Solutions for week5

week5/propositional-logic-submission.dfy
@@ -1,8 +1,8 @@
 // BEGIN-TODO(Name)
 // Please, before you do anything else, add your names here:
-// Group <Group number>
-// <Full name 1>: <Student number 1>
-// <Full name 2>: <Student number 2>
+// Group 36
+// Matilda Fogato: 1656376
+// Jip Melle Verkoulen: 1836587
 //
 // Good luck!
 //
@@ -18,13 +18,29 @@ datatype Expr =
   | Implies(left: Expr, right: Expr)
 
 // BEGIN-TODO(Extra)
-// Space for extra functions and lemmas (optional)
+function CountNodes(x: Expr): nat{
+  match x
+  case True => 1
+  case False => 1
+  case Var(s) => 1
+  case Not(arg) => 1 + CountNodes(arg)
+  case And(left, right) => 1 + CountNodes(left) + CountNodes(right)
+  case Or(left, right) => 1 + CountNodes(left) + CountNodes(right)
+  case Implies(left, right) => 1 + CountNodes(left) + CountNodes(right)
+}
 // END-TODO(Extra)
 
 predicate Eval(x: Expr, env: map<string, bool>)
 {
 // BEGIN-TODO(Eval)
-// Implement the `Eval` predicate according to the instructions.
+match x
+case True => true
+case False => false
+case Var(s) => s in env && env[s]
+case Not(arg) => !Eval(arg, env)
+case And(left, right) => Eval(left, env) && Eval(right, env)
+case Or(left, right) => Eval(left, env) || Eval(right, env)
+case Implies(left, right) => Eval(left, env) ==> Eval(right, env)
 // END-TODO(Eval)
 }
 
@@ -37,12 +53,131 @@ method TestEval()
 
 function Simplify(x: Expr): Expr
 // BEGIN-TODO(Simplify)
-// Implement the `Simplify` function according to the instructions.
+decreases CountNodes(x)
+{
+  match x {
+  case True => True
+  case False => False
+  case Var(s) => Var(s)
+  
+  case Not(arg) => 
+    var simplifiedArg := Simplify(arg);
+    match simplifiedArg {
+      case True => False
+      case False => True
+      case Not(arg1) => arg1
+      case _ => Not(simplifiedArg)
+    }
+
+  case And(left, right) =>
+    var simplifiedLeft := Simplify(left);
+    var simplifiedRight := Simplify(right);
+    match simplifiedLeft {
+    case False => False
+    case True => simplifiedRight
+    case _ =>
+      match simplifiedRight {
+      case False => False
+      case True => simplifiedLeft
+      case _ => if simplifiedLeft == simplifiedRight then simplifiedLeft else And(simplifiedLeft, simplifiedRight)
+      }
+    }
+  case Or(left, right) =>
+    var simplifiedLeft := Simplify(left);
+    var simplifiedRight := Simplify(right);
+    match simplifiedLeft {
+    case True => True
+    case False => simplifiedRight
+    case _ =>
+      match simplifiedRight {
+      case True => True
+      case False => simplifiedLeft
+      case _ => if simplifiedLeft == simplifiedRight then simplifiedLeft else Or(simplifiedLeft, simplifiedRight)
+      }
+    }
+
+  case Implies(left, right) =>
+    var simplifiedLeft := Simplify(left);
+    var simplifiedRight := Simplify(right);
+    match simplifiedLeft {
+    case True => simplifiedRight
+    case False => True
+    case _ =>
+      match simplifiedRight {
+      case True => True
+      case False => Not(simplifiedLeft)
+      case _ => Implies(simplifiedLeft, simplifiedRight)
+      }
+    }
+  }
+}
+
+//Lemma
+lemma SimplifyLemma(x: Expr, env: map<string, bool>)
+  ensures Eval(x, env) == Eval(Simplify(x), env)
+  decreases CountNodes(x)
+{
+  match x {
+  case True => 
+    assert Eval(x, env) == Eval(Simplify(x), env);
+  case False =>
+    assert Eval(x, env) == Eval(Simplify(x), env);
+  case Var(s) =>
+    assert Eval(x, env) == Eval(Simplify(x), env);
+  case Not(arg) =>
+    SimplifyLemma(arg, env);
+    assert Eval(x, env) == Eval(Simplify(x), env);
+  case And(left, right) => {
+    SimplifyLemma(left, env);
+    SimplifyLemma(right, env);
+    assert Eval(x, env) == Eval(Simplify(x), env);
+  }
+  case Or(left, right) => {
+    SimplifyLemma(left, env);
+    SimplifyLemma(right, env);
+    assert Eval(x, env) == Eval(Simplify(x), env);
+  }
+  case Implies(left, right) => {
+    SimplifyLemma(left, env);
+    SimplifyLemma(right, env);
+    assert Eval(x, env) == Eval(Simplify(x), env);
+  }
+  }
+}
 // END-TODO(Simplify)
 
 method TestSimplify()
 {
 // BEGIN-TODO(TestSimplify)
 // Insert your test cases for the `Simplify` function.
+var env := map["a" := true, "b" := false, "c" := true];
+assert Simplify(Not(Var("a"))) == Not(Var("a"));
+// True Inversion
+assert Simplify(Not(True)) == False;
+// False Inversion
+assert Simplify(Not(False)) == True;
+// Double Negation
+assert Simplify(Not(Not(Var("a")))) == Var("a");
+// Idempotence
+assert Simplify(And(Var("a"), Var("a"))) == Var("a");
+assert Simplify(Or(Var("a"), Var("a"))) == Var("a");
+// True - Elim
+assert Simplify(And(Var("a"), True)) == Var("a");
+assert Simplify(Or(Var("a"), True)) == True;
+assert Simplify(And(True, Var("a"))) == Var("a");
+assert Simplify(Or(True, Var("a"))) == True;
+// False - Elim
+assert Simplify(And(Var("a"), False)) == False;
+assert Simplify(Or(Var("a"), False)) == Var("a");
+assert Simplify(And(False, Var("a"))) == False;
+assert Simplify(Or(False, Var("a"))) == Var("a");
+// Implication cases
+assert Simplify(Implies(True, Var("a"))) == Var("a");
+assert Simplify(Implies(False, Var("a"))) == True;
+assert Simplify(Implies(Var("a"), True)) == True;
+assert Simplify(Implies(Var("a"), False)) == Not(Var("a"));
+// Complex Cases
+assert Simplify(And(Or(Var("a"), False), Not(Not(Var("b"))))) == And(Var("a"), Var("b"));
+assert Simplify(Or(And(Var("a"), True), And(False, Var("b")))) == Var("a");
 // END-TODO(TestSimplify)
 }
