week5/mirror-submission.dfy
@@ -1,8 +1,8 @@
 // BEGIN-TODO(Name)
 // Please, before you do anything else, add your names here:
-// Group <Group number>
-// <Full name 1>: <Student number 1>
-// <Full name 2>: <Student number 2>
+// Group 36
+// Matilda Fogato: 1656376
+// Jip Melle Verkoulen: 1836587
 //
 // Good luck!
 //
@@ -19,7 +19,10 @@ datatype BYTree = BlueLeaf
 function Mirror(t: BYTree): BYTree
 {
 // BEGIN-TODO(Mirror)
-// Implement the `Mirror` predicate according to the instructions.
+    match t
+    case BlueLeaf => BlueLeaf
+    case YellowLeaf => YellowLeaf
+    case Node(left, right) => Node(Mirror(right), Mirror(left))
 // END-TODO(Mirror)
 }
 
